coq/JsPrettyRules.v
@@ -1667,7 +1667,7 @@ with red_expr : state -> execution_ctx -> ext_expr -> out -> Prop :=
 
   (** HasProperty (8.12.6) *)
 
-  | red_spec_object_has_prop_1_default : forall o1 (* This [o1] should be removed -- Martin. *) S C l x o, (* Step 1 *)
+  | red_spec_object_has_prop_1_default : forall S C l x o, (* Step 1 *)
       red_expr S C (spec_object_get_prop l x spec_object_has_prop_2) o ->
       red_expr S C (spec_object_has_prop_1 builtin_has_prop_default l x) o  
 
@@ -2352,7 +2352,7 @@ with red_expr : state -> execution_ctx -> ext_expr -> out -> Prop :=
       red_expr S C (spec_binding_inst_var_decls_1 L vd vds bconfig str o1) o ->
       red_expr S0 C (spec_binding_inst_var_decls L (vd::vds) bconfig str) o (* I think this [S0] should be removed of this rule, and in the following three. -- Martin. *)
 
-  | red_spec_binding_inst_var_decls_1_true : forall o1 L S0 S C vd vds bconfig str o, (* Step 8c *)
+  | red_spec_binding_inst_var_decls_1_true : forall L S0 S C vd vds bconfig str o, (* Step 8c *)
       red_expr S C (spec_binding_inst_var_decls L vds bconfig str) o ->
       red_expr S0 C (spec_binding_inst_var_decls_1 L vd vds bconfig str (out_ter S true)) o
 
@@ -2408,16 +2408,16 @@ with red_expr : state -> execution_ctx -> ext_expr -> out -> Prop :=
       red_expr S C (spec_binding_inst_7 code bconfig L o1) o ->
       red_expr S0 C (spec_binding_inst_6 codetype_func (Some lf) code xs args bconfig L (out_ter S false)) o
       
-  | red_spec_binding_inst_7 : forall o1 L S C code bconfig L o, (* Step 7, continued *)
+  | red_spec_binding_inst_7 : forall L S C code bconfig L o, (* Step 7, continued *)
       red_expr S C (spec_binding_inst_8 code bconfig L) o ->
       red_expr S C (spec_binding_inst_7 code bconfig L (out_void S)) o
 
-  | red_spec_binding_inst_6_no_arguments : forall o1 L S0 S C ct olf code xs args bconfig bdefined o, (* Step 7 not needed *) 
+  | red_spec_binding_inst_6_no_arguments : forall L S0 S C ct olf code xs args bconfig bdefined o, (* Step 7 not needed *) 
       ~ (ct = codetype_func /\ bdefined = true) ->
       red_expr S C (spec_binding_inst_8 code bconfig L) o ->
       red_expr S0 C (spec_binding_inst_6 ct olf code xs args bconfig L (out_ter S bdefined)) o
 
-  | red_spec_binding_inst_8 : forall o1 S0 L S C code bconfig o, (* Step 8 *)
+  | red_spec_binding_inst_8 : forall S0 L S C code bconfig o, (* Step 8 *)
       red_expr S C (spec_binding_inst_var_decls L (prog_vardecl code) bconfig (prog_intro_strictness code)) o ->
       red_expr S0 C (spec_binding_inst_8 code bconfig L) o
 
